---
layout: post
title: First post
published: true
---

Hiya there, It's sammy. 
$$\sigma + \alpha = \frac{\sigma\alpha}{2}$$
Hiya there, It's sammy. $$\sigma + \alpha = \frac{\sigma\alpha}{2}$$Hiya there, It's sammy. $$\sigma + \alpha = \frac{\sigma\alpha}{2}$$Hiya there, It's sammy. $$\sigma + \alpha = \frac{\sigma\alpha}{2}$$Hiya there, It's sammy. $$\sigma + \alpha = \frac{\sigma\alpha}{2}$$Hiya there, It's sammy. $$\sigma + \alpha = \frac{\sigma\alpha}{2}$$Hiya there, It's sammy. $$\sigma + \alpha = \frac{\sigma\alpha}{2}$$Hiya there, It's sammy. $$\sigma + \alpha = \frac{\sigma\alpha}{2}$$Hiya there, It's sammy. $$\sigma + \alpha = \frac{\sigma\alpha}{2}$$Hiya there, It's sammy. $$\sigma + \alpha = \frac{\sigma\alpha}{2}$$Hiya there, It's sammy. $$\sigma + \alpha = \frac{\sigma\alpha}{2}$$Hiya there, It's sammy. $$\sigma + \alpha = \frac{\sigma\alpha}{2}$$Hiya there, It's sammy. $$\sigma + \alpha = \frac{\sigma\alpha}{2}$$Hiya there, It's sammy. $$\sigma + \alpha = \frac{\sigma\alpha}{2}$$Hiya there, It's sammy. $$\sigma + \alpha = \frac{\sigma\alpha}{2}$$Hiya there, It's sammy. $$\sigma + \alpha = \frac{\sigma\alpha}{2}$$Hiya there, It's sammy. $$\sigma + \alpha = \frac{\sigma\alpha}{2}$$Hiya there, It's sammy. $$\sigma + \alpha = \frac{\sigma\alpha}{2}$$Hiya there, It's sammy. $$\sigma + \alpha = \frac{\sigma\alpha}{2}$$Hiya there, It's sammy. $$\sigma + \alpha = \frac{\sigma\alpha}{2}$$Hiya there, It's sammy. $$\sigma + \alpha = \frac{\sigma\alpha}{2}$$Hiya there, It's sammy. $$\sigma + \alpha = \frac{\sigma\alpha}{2}$$Hiya there, It's sammy. $$\sigma + \alpha = \frac{\sigma\alpha}{2}$$Hiya there, It's sammy. $$\sigma + \alpha = \frac{\sigma\alpha}{2}$$Hiya there, It's sammy. $$\sigma + \alpha = \frac{\sigma\alpha}{2}$$Hiya there, It's sammy. $$\sigma + \alpha = \frac{\sigma\alpha}{2}$$Hiya there, It's sammy. $$\sigma + \alpha = \frac{\sigma\alpha}{2}$$Hiya there, It's sammy. $$\sigma + \alpha = \frac{\sigma\alpha}{2}$$Hiya there, It's sammy. $$\sigma + \alpha = \frac{\sigma\alpha}{2}$$Hiya there, It's sammy. $$\sigma + \alpha = \frac{\sigma\alpha}{2}$$Hiya there, It's sammy. $$\sigma + \alpha = \frac{\sigma\alpha}{2}$$Hiya there, It's sammy. $$\sigma + \alpha = \frac{\sigma\alpha}{2}$$Hiya there, It's sammy. $$\sigma + \alpha = \frac{\sigma\alpha}{2}$$Hiya there, It's sammy. $$\sigma + \alpha = \frac{\sigma\alpha}{2}$$Hiya there, It's sammy. $$\sigma + \alpha = \frac{\sigma\alpha}{2}$$Hiya there, It's sammy. $$\sigma + \alpha = \frac{\sigma\alpha}{2}$$Hiya there, It's sammy. $$\sigma + \alpha = \frac{\sigma\alpha}{2}$$Hiya there, It's sammy. $$\sigma + \alpha = \frac{\sigma\alpha}{2}$$Hiya there, It's sammy. $$\sigma + \alpha = \frac{\sigma\alpha}{2}$$Hiya there, It's sammy. $$\sigma + \alpha = \frac{\sigma\alpha}{2}$$Hiya there, It's sammy. $$\sigma + \alpha = \frac{\sigma\alpha}{2}$$Hiya there, It's sammy. $$\sigma + \alpha = \frac{\sigma\alpha}{2}$$Hiya there, It's sammy. $$\sigma + \alpha = \frac{\sigma\alpha}{2}$$Hiya there, It's sammy. $$\sigma + \alpha = \frac{\sigma\alpha}{2}$$Hiya there, It's sammy. $$\sigma + \alpha = \frac{\sigma\alpha}{2}$$Hiya there, It's sammy. $$\sigma + \alpha = \frac{\sigma\alpha}{2}$$Hiya there, It's sammy. $$\sigma + \alpha = \frac{\sigma\alpha}{2}$$Hiya there, It's sammy. $$\sigma + \alpha = \frac{\sigma\alpha}{2}$$Hiya there, It's sammy. $$\sigma + \alpha = \frac{\sigma\alpha}{2}$$Hiya there, It's sammy. $$\sigma + \alpha = \frac{\sigma\alpha}{2}$$Hiya there, It's sammy. $$\sigma + \alpha = \frac{\sigma\alpha}{2}$$Hiya there, It's sammy. $$\sigma + \alpha = \frac{\sigma\alpha}{2}$$Hiya there, It's sammy. $$\sigma + \alpha = \frac{\sigma\alpha}{2}$$Hiya there, It's sammy. $$\sigma + \alpha = \frac{\sigma\alpha}{2}$$Hiya there, It's sammy. $$\sigma + \alpha = \frac{\sigma\alpha}{2}$$Hiya there, It's sammy. $$\sigma + \alpha = \frac{\sigma\alpha}{2}$$Hiya there, It's sammy. $$\sigma + \alpha = \frac{\sigma\alpha}{2}$$Hiya there, It's sammy. $$\sigma + \alpha = \frac{\sigma\alpha}{2}$$
